Remove misleading `LawfulGenerator` class
The LawfulGenerator class overstated the degree to which those three
laws were the "right" ones. In practice, users should mix and match.

Basalt/Laws.lean
@@ -9,10 +9,10 @@ import Basalt.SPMF.Cost
 import Basalt.SPMF.Failure
 
 /-!
-# Generator Correctness Classes
+# Generator Correctness Properties
 
-The classes in this file encode the basic, mostly orthogonal, correctness properties that we expect
-of an optimal PBT generator.
+The definitions in this file encode basic, mostly orthogonal, correctness properties that a PBT
+generator may have. Which of them apply depends on the generator.
 
 ## Main Definitions
 
@@ -26,33 +26,30 @@ of an optimal PBT generator.
 - `IsCostBounded` — We expect that a generator makes a bounded number of choices while producing a
   given value. For example, we may expect that a generator for BSTs makes roughly `t.size` choices
   to produce a tree `t`.
-- `LawfulGenerator` — A generator that is all of the above is _lawful_.
 -/
 
 /-- We say that a generator `g` `IsSoundAndComplete` with respect to a predicate `P` if, when
   interpreted as an `SPMF`, all values in the support of `g` satisfy `P` and all values satisfying
   `P` are in the support of `g`. -/
-class IsSoundAndComplete (g : SPMF α) (P : α → Prop) where
-  support_iff : a ∈ SPMF.support g ↔ P a
+def IsSoundAndComplete (g : SPMF α) (P : α → Prop) : Prop :=
+  ∀ a, a ∈ SPMF.support g ↔ P a
 
 /-- We say that a generator `g` `IsAlmostSurelyTerminating` if, when
   interpreted as an `SPMF`, its mass sums to 1 (i.e., it is a true `PMF`). -/
-class IsAlmostSurelyTerminating (g : SPMF α) where
-  is_pmf : SPMF.IsPMF g
+def IsAlmostSurelyTerminating (g : SPMF α) : Prop :=
+  SPMF.IsPMF g
 
 /-- We say that a generator `g` `IsCostBounded` with respect to a cost function `c` if, when
   generating a value `v`, the generator makes at most `c v` choices. -/
-class IsCostBounded (g : SPMF.Cost α) (c : α → Nat) where
-  is_bounded : IsBounded g c
-
-class LawfulGenerator (g : ∀ {G : Type → Type} [Gen G], G α) (P : α → Prop) (c : α → Nat) extends IsSoundAndComplete g P, IsAlmostSurelyTerminating g, IsCostBounded g c
+def IsCostBounded (g : SPMF.Cost α) (c : α → Nat) : Prop :=
+  IsBounded g c
 
 /-- A partial generator `IsFilterFree` if all of its mass lands on *successful* outcomes: it never
   actually fails.  -/
-class IsFilterFree (g : SPMF (Option α)) where
-  filter_free : SPMF.massSome g = 1
+def IsFilterFree (g : SPMF (Option α)) : Prop :=
+  SPMF.massSome g = 1
 
 /-- A partial generator `IsProductive` if it succeeds with positive probability.  Proving this shows
   that rejection sampling is safe. -/
-class IsProductive (g : SPMF (Option α)) where
-  productive : 0 < SPMF.massSome g
+def IsProductive (g : SPMF (Option α)) : Prop :=
+  0 < SPMF.massSome g
