BasaltExamples/ArbChar.lean
@@ -10,18 +10,22 @@ private theorem alphanumChars_eq_filter :
     ∀ c : Char, c ∈ alphanumChars ↔ c.isAlphanum = true := by native_decide
 
 /-- All alphanumeric characters are generable by `Char.arbitrary` -/
-theorem Char.arbitrary_support :
+theorem Char.arbitrary_mem_support :
     c ∈ SPMF.support Char.arbitrary ↔ c.isAlphanum = true := by
   rw [Char.arbitrary, SPMF.mem_support_elements_iff]
   exact alphanumChars_eq_filter c
 
+theorem Char.arbitrary_support :
+    IsSoundAndComplete Char.arbitrary (fun c => c.isAlphanum = true) :=
+  fun _ => Char.arbitrary_mem_support
+
 /-- `Char.arbitrary` almost surely terminates -/
-theorem Char.arbitrary_terminates : SPMF.IsPMF Char.arbitrary := by
+theorem Char.arbitrary_terminates : IsAlmostSurelyTerminating Char.arbitrary := by
   unfold Char.arbitrary
   apply SPMF.IsPMF_elements
 
 theorem Char.arbitrary_cost :
-    IsBounded Char.arbitrary (fun _ => 1) := by
+    IsCostBounded Char.arbitrary (fun _ => 1) := by
   unfold Char.arbitrary
   exact IsBounded_elements _
 
